\documentclass[11pt, oneside]{article}   	% use "amsart" instead of "article" for AMSLaTeX format
\usepackage{geometry}                		% See geometry.pdf to learn the layout options. There are lots.
\geometry{letterpaper}                   		% ... or a4paper or a5paper or ... 
%\geometry{landscape}                		% Activate for for rotated page geometry
%\usepackage[parfill]{parskip}    		% Activate to begin paragraphs with an empty line rather than an indent
\usepackage{graphicx}				% Use pdf, png, jpg, or epsÂ§ with pdflatex; use eps in DVI mode
								% TeX will automatically convert eps --> pdf in pdflatex		
\usepackage{amssymb}

\title{HW 3.3 }
\author{Rob Navarro}
%\date{}							% Activate to display a given date or no date

\begin{document}
\maketitle
%\section{}
%\subsection{}

\noindent
4. What are the terms $a_0, a_1, a_2$, and $a_3$ of the sequence $\{a_n\}$, where $a_n$ equals: \\\\
a) $(-2)^n: 1, -2, 4, -8$\\
b) $3: 3, 3, 3, 3$\\
c) $7 + 4^n: 8, 11, 23, 71$\\
d) $2^n + (-2)^n: 2, 0, 8, 0$\\\\
29. What are the values of these sums?\\\\
a) $\sum\limits_{k=1}^5 (k + 1) = 2 + 3 + 4 + 5 + 6 = 20$\\
b) $\sum\limits_{j=0}^4 (-2)^j = 1 - 2 + 4 - 8 + 16 = 11$\\
c) $\sum\limits_{i=1}^10 3 = 10 * 3 = 30$\\
d) $\sum\limits_{j=0}^8 (2^{j+1} - 2^j) = \sum\limits_{j=0}^8 2^j = \frac{2^9 - 2^0}{2 - 1} = 511$\\\\
31. What is the value of each of these sums of terms of geometric progression?\\\\
a) $\sum\limits_{j=0}^8 3 * 2^j = 3*\frac{2^9 - 2^0}{2 - 1}= 1533\\$
b) $\sum\limits_{j=1}^8 2^j = \sum\limits_{j=0}^8 2^j - \sum\limits_{j=0}^0 2^j = \frac{2^9 - 2^0}{2 - 1} - \frac{2^1 - 2^0}{2 - 1} = 511 - 1 = 510$\\\\
c) $\sum\limits_{j=2}^8 (-3)^j = \sum\limits_{j=0}^8 (-3)^j - \sum\limits_{j=0}^1 (-3)^j = \frac{(-3)^9 - (-3)^0}{-3 - 1} - \frac{(-3)^2 - (-3)^0}{-3 - 1}$ = 4923\\
d) $\sum\limits_{j=2}^8 2*(-3)^j = 2\sum\limits_{j=2}^8 (-3)^j = 2*\frac{(-3)^9 - (-3)^0}{-3 - 1} = 2 * 4921 = 9842$\\\\
32. Find the value of each of these sums.\\\\
a) $\sum\limits_{j=0}^8 (1 + (-1)^j) = 2 + 0 + 2 + 0 + 2 + 0 + 2 + 0 + 2 = 10\\$
b) $\sum\limits_{j=0}^8 (3^j - 2^j) = \sum\limits_{j=0}^8 3^j - \sum\limits_{j=0}^8 2^j = \frac{(3)^9 - (3)^0}{3 - 1} - \frac{(2)^9 - (2)^0}{2 - 1} = 9841 - 511 = 9330$\\
c) $\sum\limits_{j=0}^8 (2 * 3^j + 3 * 2^j) = 2*\sum\limits_{j=0}^8 3^j + 3*\sum\limits_{j=0}^8 2^j = 2*\frac{(3)^9 - (3)^0}{3 - 1} - 3*\frac{(2)^9 - (2)^0}{2 - 1} = 19682 + 1533 = 21215$\\
d) $\sum\limits_{j=0}^8 (2^{j + 1} - 2^j) = \sum\limits_{j=0}^8 2^j(2 - 1) = \sum\limits_{j=0}^8 2^j = \frac{2^9 - 2^0}{2 - 1} = 511$\\\\
34. Compute each of these double sums.\\\\
a) $\sum\limits_{i=1}^3 \sum\limits_{j=1}^2 (i - j) = \sum\limits_{i=1}^3 (\sum\limits_{j=1}^2 i - \sum\limits_{j=1}^2 j) = 2*\sum\limits_{i=1}^3 i - \sum\limits_{i=1}^3 3 = 2(1 + 2 + 3) - 3 * 3 = 3$\\
b) $\sum\limits_{i=0}^3 \sum\limits_{j=0}^2 (3i + 2j) = \sum\limits_{i=0}^3 (3*\sum\limits_{j=0}^2 i + 2*\sum\limits_{j=0}^2 j) = \sum\limits_{i=0}^3 (9i + 6) = 9*(0 + 1 + 2 + 3) + 6 * 4 = 78$\\
c) $\sum\limits_{i=0}^3 \sum\limits_{j=0}^2 j = \sum\limits_{i=0}^3 3 = 9$\\
d) $\sum\limits_{i=0}^2 \sum\limits_{j=0}^3 i^2j^3 = \sum\limits_{i=0}^2 i^2 \sum\limits_{j=0}^3 j^3 = 5 * 36 = 180$\\\\
36. Use the identity $\frac{1}{k(k + 1) }= \frac{1}{k} - \frac{1}{k + 1}$ and exercise 19 to compute $\sum\limits_{k=1}^n \frac{1}{k(k + 1)}$.\\\\
$\sum\limits_{k=1}^n \frac{1}{k(k + 1)} = (1 - \frac{1}{2}) + (\frac{1}{2} - \frac{2}{3})... + (\frac{1}{n} - \frac{1}{n + 1})$\\
Let $a_k = \frac{1}{k}$
Then using the conclusion from exercise 19 we know $\sum\limits_{j=1}^n (a_j - a_{n+1}) = a_1 - a_{n+1}$.
With this in mind we now know $\sum\limits_{k=1}^n \frac{1}{k(k + 1)} = \frac{n}{n + 1}$\\\\
40. Find $\sum\limits_{k=99}^200 k^3$.\\\\
$\sum\limits_{k=99}^{200} k^3 = \sum\limits_{k=1}^{200} k^3 - \sum\limits_{k=1}^{98} k^3 = \frac{200^2 * 201^2}{4} - \frac{98^2 * 99^2}{4} = 380477799$\\



\end{document}  